proper eval apply machine generation

refocusing_lang.v
@@ -241,11 +241,13 @@ Module Type ABSTRACT_MACHINE.
   Parameter transition : configuration -> configuration -> Prop.
 
   Inductive trans_close : configuration -> configuration -> Prop :=
-  | one_step   : forall (c0 c1 : configuration), transition c0 c1 -> trans_close c0 c1
-  | multi_step : forall (c0 c1 c2 : configuration), transition c0 c1 -> trans_close c1 c2 -> trans_close c0 c2.
+  | one_step   : forall (c0 c1 : configuration), 
+                     transition c0 c1 -> trans_close c0 c1
+  | multi_step : forall (c0 c1 c2 : configuration), 
+                     transition c0 c1 -> trans_close c1 c2 -> trans_close c0 c2.
 
   Inductive eval : term -> value -> Prop :=
-  | e_intro : forall (t : term) (v : value), trans_close (c_init t) (c_final v) -> eval t v.
+  | e_intro : forall t v, trans_close (c_init t) (c_final v) -> eval t v.
 
 End ABSTRACT_MACHINE.
 
