refocusing_signatures.v
@@ -28,17 +28,19 @@ Module Type RED_SEM (R : RED_LANG).
                            ~ dead_ckind k2 ->  dec t (c ~+ c0) d -> 
                            dec c[t] c0 d.
 
+
   Inductive decempty : term -> forall {k}, decomp k -> Prop :=
   | d_intro : forall {t k} {d : decomp k}, dec t [_] d -> decempty t d.
 
   Inductive iter : forall {k}, decomp k -> value k -> Prop :=
   | i_val : forall {k} (v : value k), iter (d_val v) v
   | i_red : forall {k2} (r : redex k2) {t k1} (c : context k1 k2) {d v},
-              contract r = Some t -> decempty c[t] d -> iter d v ->
-              iter (d_red r c) v.
+                contract r = Some t -> decempty c[t] d -> iter d v ->
+                iter (d_red r c) v.
 
-  Inductive eval : term -> forall {k}, value k -> Prop :=
-  | e_intro : forall {t k} {d : decomp k} {v}, decempty t d -> iter d v -> eval t v.
+  Inductive eval : term -> value init_ckind -> Prop :=
+  | e_intro : forall {t} {d : decomp init_ckind} {v : value init_ckind}, 
+                  decempty t d -> iter d v -> eval t v.
 
 End RED_SEM.
 
@@ -73,6 +75,12 @@ Module Type RED_REF_SEM (R : RED_LANG).
   Axiom dec_term_next_alive : 
       forall t k {t0 ec0}, dec_term t k = in_term t0 ec0 -> ~ dead_ckind (k+>ec0).
 
+  Axiom dec_term_from_dead : 
+      forall t k, dead_ckind k -> dec_term t k = in_dead k.
+
+  Axiom dec_context_from_dead : 
+      forall ec k (v : value (k+>ec)), 
+          dead_ckind (k+>ec) -> dec_context ec k v = in_dead k.
 
   (** A decomposition function specified in terms of the atomic functions above *)
   Inductive dec : term -> forall {k1 k2}, context k1 k2 -> decomp k1 -> Prop :=
@@ -144,7 +152,7 @@ Module Type RED_SEM_PROPER (R : RED_LANG) (RS : RED_SEM R).
                                decempty t d -> decempty t d0 -> d = d0.
   Axiom iter_is_function : forall {k} {d : decomp k} {v v0}, 
                                iter d v -> iter d v0 -> v = v0.
-  Axiom eval_is_function : forall {t k} {v v0 : value k}, 
+  Axiom eval_is_function : forall {t} {v v0 : value init_ckind}, 
                                eval t v -> eval t v0 -> v = v0.
   Axiom dec_correct      : forall {t k1 k2} {c : context k1 k2} {d},
                                dec t c d -> decomp_to_term d = plug t c.
@@ -223,14 +231,15 @@ Module Type PRE_ABSTRACT_MACHINE (R : RED_LANG).
   Scheme dec_Ind := Induction for dec Sort Prop
     with decctx_Ind := Induction for decctx Sort Prop.
 
+
   Inductive iter : forall {k}, decomp k -> value k -> Prop :=
   | i_val : forall {k} (v : value k), iter (d_val v) v
   | i_red : forall {k2} (r : redex k2) {t k1} {c : context k1 k2} {d v},
               contract r = Some t -> dec t c d -> iter d v ->
               iter (d_red r c) v.
 
-  Inductive eval : term -> forall {k}, value k -> Prop :=
-  | e_intro : forall {t k} {d : decomp k} {v},
+  Inductive eval : term -> value init_ckind -> Prop :=
+  | e_intro : forall {t} {d : decomp init_ckind} {v : value init_ckind},
                 dec t [_] d -> iter d v -> eval t v.
 
 End PRE_ABSTRACT_MACHINE.
@@ -275,18 +284,18 @@ Module Type STAGED_ABSTRACT_MACHINE (R : RED_LANG).
 
   with decctx : forall {k2}, value k2 -> forall {k1}, context k1 k2 -> value k1 -> Prop :=
   | dc_end  : forall {k} {v v0 : value k},
-               ~ dead_ckind k ->
-               iter (d_val v) v0 ->
-               decctx v [_] v0
+                ~ dead_ckind k ->
+                iter (d_val v) v0 ->
+                decctx v [_] v0
   | dc_dec  : forall ec {k2} (v : value (k2+>ec)) {k1} {c : context k1 k2} {r v0},
-               dec_context ec k2 v = in_red r -> iter (d_red r c) v0 ->
-               decctx v (ec=:c) v0
+                dec_context ec k2 v = in_red r -> iter (d_red r c) v0 ->
+                decctx v (ec=:c) v0
   | dc_val  : forall ec {k2} (v : value (k2+>ec)) {v0 k1} {c : context k1 k2} {v1},
-               dec_context ec k2 v = in_val v0 -> decctx v0 c v1 ->
-               decctx v (ec=:c) v1
+                dec_context ec k2 v = in_val v0 -> decctx v0 c v1 ->
+                decctx v (ec=:c) v1
   | dc_term : forall ec {k2} (v : value (k2+>ec)) {t ec0 k1} {c : context k1 k2} {v0},
-               dec_context ec k2 v = in_term t ec0 -> dec t (ec0=:c) v0 ->
-               decctx v (ec=:c) v0
+                dec_context ec k2 v = in_term t ec0 -> dec t (ec0=:c) v0 ->
+                decctx v (ec=:c) v0
 
   with iter : forall {k}, decomp k -> value k -> Prop :=
   | i_val : forall {k} (v : value k), 
@@ -299,8 +308,9 @@ Module Type STAGED_ABSTRACT_MACHINE (R : RED_LANG).
     with decctx_Ind := Induction for decctx Sort Prop
     with iter_Ind   := Induction for iter Sort Prop.
 
-  Inductive eval : term -> forall {k}, value k -> Prop :=
-  | e_intro : forall {t k} {v : value k}, dec t [_] v -> eval t v.
+
+  Inductive eval : term -> value init_ckind -> Prop :=
+  | e_intro : forall {t} {v : value init_ckind}, dec t [_] v -> eval t v.
 
 End STAGED_ABSTRACT_MACHINE.
 
@@ -361,7 +371,82 @@ Module Type EVAL_APPLY_MACHINE (R : RED_LANG).
     with decctx_Ind := Induction for decctx Sort Prop.
 
 
-  Inductive eval : term -> forall {k}, value k -> Prop :=
-  | e_intro : forall {t k} {v : value k}, dec t [_] v -> eval t v.
+  Inductive eval : term -> value init_ckind -> Prop :=
+  | e_intro : forall {t} {v : value init_ckind}, dec t [_] v -> eval t v.
 
 End EVAL_APPLY_MACHINE.
+
+
+
+Module Type PROPER_EA_MACHINE (R : RED_LANG).
+
+  Import R.
+
+  (** Functions specifying atomic steps of induction on terms and contexts -- needed to avoid explicit induction on terms and contexts in construction of the AM *)
+  Parameter dec_term    : term -> forall k, interm_dec k.
+  Parameter dec_context : forall ec k, value (k+>ec) -> interm_dec k.
+
+  Axiom dec_term_correct : 
+      forall t k, match dec_term t k with
+      | in_red r       => t = r
+      | in_val v       => t = v
+      | in_term t0 ec0 => t = ec0:[t0]
+      | in_dead        => dead_ckind k
+      end.
+
+  Axiom dec_context_correct : 
+      forall ec k v, match dec_context ec k v with
+      | in_red r      => ec:[v] = r
+      | in_val v0     => ec:[v] = v0
+      | in_term t ec0 => ec:[v] = ec0:[t]
+      | in_dead       => dead_ckind (k+>ec) 
+      end.
+
+  Inductive configuration : Set :=
+  | c_eval  : term -> forall {k1 k2}, context k1 k2 -> configuration
+  | c_apply : forall {k1 k2}, context k1 k2 -> value k2 -> configuration.
+(*  | c_final : value init_ckind -> configuration.*)
+
+  Definition c_init t                       := c_eval t (@empty init_ckind).
+  Definition c_final (v : value init_ckind) := c_apply [_] v.
+
+
+  Reserved Notation " a → b " (at level 40, no associativity).
+
+
+  Inductive transition : configuration -> configuration -> Prop :=
+(*  | t_init : forall t, 
+               c_init t → c_eval t (@empty init_ckind)*)
+  | t_red  : forall t {k1 k2} (c : context k1 k2) {r t0},
+               dec_term t k2 = in_red r -> contract r = Some t0 ->
+               c_eval t c → c_eval t0 c
+  | t_val  : forall t {k1 k2} (c : context k1 k2) {v},
+      	       dec_term t k2 = in_val v ->
+               c_eval t c → c_apply c v
+  | t_term : forall t {k1 k2} (c : context k1 k2) {t0 ec},
+               dec_term t k2 = in_term t0 ec ->
+               c_eval t c → c_eval t0 (ec=:c)
+(*  | t_cfin : forall (v : value init_ckind),
+               ~ dead_ckind init_ckind ->
+               c_apply [_] v → c_final v*)
+  | t_cred : forall ec {k2} (v : value (k2+>ec)) {k1} (c : context k1 k2) {r t},
+               dec_context ec k2 v = in_red r -> contract r = Some t ->
+               c_apply (ec=:c) v → c_eval t c
+  | t_cval : forall ec {k2} (v : value (k2+>ec)) {k1} (c : context k1 k2) {v0},
+               dec_context ec k2 v = in_val v0 ->
+               c_apply (ec=:c) v → c_apply c v0
+  | t_cterm: forall ec {k2} (v : value (k2+>ec)) {k1} (c : context k1 k2) {t ec0},
+               dec_context ec k2 v = in_term t ec0 ->
+               c_apply (ec=:c) v → c_eval t (ec0=:c)
+  where " a → b " := (transition a b).
+
+
+  Declare Module AM : ABSTRACT_MACHINE
+    with Definition term := term
+    with Definition value := value init_ckind
+    with Definition configuration := configuration
+    with Definition transition := transition
+    with Definition c_init := c_init
+    with Definition c_final := c_final.
+
+End PROPER_EA_MACHINE.
